Proved quiesce_request, except a bit of ineq reasoning;
should use quiesce_request upon crash to satisfy the crash condition.

Statement is not quite right; need to know that if some other unrelated
RPC is done after crashing, we can still take the resources of the
earlier failed RPC. Seems like it should be more like idemp_fupd2.

src/program_proof/lockservice/incr_proof.v
@@ -257,14 +257,14 @@ Context `{!heapG Σ}.
 Context `{!rpcG Σ u64}.
 
 (* TODO: come up with proper names for these things *)
-Definition IdempotentPre2 γrpc (cid seq:u64) (PreCond : RPCValC → iProp Σ) : (RPCValC → iProp Σ) :=
+Definition IdempotentPre2 γrpc (cid seq:u64) (PreCond : RPCValC → iProp Σ) (PostCond:RPCValC → u64 → iProp Σ) : (RPCValC → iProp Σ) :=
   λ (args:RPCValC),
-        (own γrpc.(proc) (Excl ()) -∗ cid fm[[γrpc.(lseq)]]≥ int.nat seq ={⊤}=∗ own γrpc.(proc) (Excl ()) ∗ PreCond args)%I.
+        (own γrpc.(proc) (Excl ()) -∗ cid fm[[γrpc.(lseq)]]≥ int.nat seq ={⊤}=∗ own γrpc.(proc) (Excl ()) ∗ ▷ (PreCond args ∨ (∃ reply,PostCond args reply)))%I.
 
-Definition idemp_fupd2 γrpc cid args PreCond : iProp Σ :=
+Definition idemp_fupd2 γrpc cid args PreCond PostCond : iProp Σ :=
     <bdisc> (∀ seq, cid fm[[γrpc.(cseq)]]↦ seq ={⊤}=∗
       cid fm[[γrpc.(cseq)]]↦ seq ∗
-    IdempotentPre2 γrpc cid seq PreCond args)
+    IdempotentPre2 γrpc cid seq PreCond PostCond args)
 .
 
 Definition own_rpcclient (cl_ptr:loc) (γrpc:rpc_names) (cid:u64) : iProp Σ
@@ -313,8 +313,63 @@ Proof.
     by iLeft in "H".
 Qed.
 
+Lemma quiesce_request E (req:RPCRequest) new_seq γrpc γreq PreCond PostCond :
+  ↑rpcRequestInvN ⊆ E →
+  ↑replyTableInvN ⊆ E →
+  (int.nat new_seq > int.nat req.(Req_Seq)) →
+  is_RPCServer γrpc -∗
+  is_RPCRequest γrpc γreq PreCond PostCond req -∗
+  (RPCRequest_token γreq) ={E}=∗
+  IdempotentPre2 γrpc req.(Req_CID) new_seq PreCond PostCond req.(Req_Args).
+Proof.
+    iIntros (Hnamespace1 Hnamespace2 Hnew_seq) "#Hsrpc #His_req Hγpost".
+    iModIntro.
+
+    iIntros "Hγproc #Hlseq_lb".
+    iInv "His_req" as "HN" "HNClose".
+    iDestruct "HN" as "[#>Hcseq_lb_strict [HN|HN]]"; simpl. (* Is cseq_lb_strict relevant for this? *)
+    {
+      iDestruct "HN" as "[_ [>Hbad|HN]]".
+      { iDestruct (own_valid_2 with "Hbad Hγproc") as %?; contradiction. }
+
+      (* iInv "Hsrpc" as ">HM" "HMClose".
+      iNamed "HM". *)
+
+      iMod ("HNClose" with "[Hγpost]") as "_".
+      { iNext. iFrame "Hcseq_lb_strict". iRight. iFrame.
+        iSplitR ""; last admit.
+        admit.
+        (* TODO: fmcounter reasoning *)
+      }
+      iFrame.
+      iModIntro.
+      iNext.
+      iLeft.
+      iDestruct "HN" as "[_ $]".
+    }
+    {
+      iDestruct "HN" as "[_ HN]".
+      iDestruct "HN" as (last_reply) "[#>Hreply [>Hbad | HP]]".
+      { by iDestruct (own_valid_2 with "Hγpost Hbad") as %Hbad. }
+      iMod ("HNClose" with "[Hγpost]") as "_".
+      {
+        iNext.
+        iFrame "Hcseq_lb_strict".
+        iRight.
+        iFrame "# ∗".
+        iSplitL "Hlseq_lb".
+        { admit. (* Use Hnew_seq and Hlseq_lb *) }
+        iExists _; iFrame "Hreply".
+      }
+      iModIntro.
+      iFrame.
+      iRight.
+      iExists _; iFrame.
+    }
+Admitted.
+
 Lemma wpc_RPCClient__MakeRequest k E (f:goose_lang.val) cl_ptr cid args γrpc (PreCond:RPCValC -> iProp Σ) PostCond {_:Discretizable (PreCond args)}:
-  (∀ seqno, is_rpcHandler f γrpc (IdempotentPre2 γrpc cid seqno PreCond) PostCond) -∗
+  (∀ seqno, is_rpcHandler f γrpc (IdempotentPre2 γrpc cid seqno PreCond PostCond) PostCond) -∗
   {{{
     PreCond args ∗
     own_rpcclient cl_ptr γrpc cid ∗
@@ -322,7 +377,7 @@ Lemma wpc_RPCClient__MakeRequest k E (f:goose_lang.val) cl_ptr cid args γrpc (P
   }}}
     RPCClient__MakeRequest #cl_ptr f (into_val.to_val args) @ k ; E
   {{{ (retv:u64), RET #retv; own_rpcclient cl_ptr γrpc cid ∗ PostCond args retv }}}
-  {{{ idemp_fupd2 γrpc cid args PreCond }}}.
+  {{{ idemp_fupd2 γrpc cid args PreCond PostCond }}}.
 Proof using Type*.
   iIntros "#Hfspec" (Φ Φc) "!# [Hprecond [Hclerk #Hlinv]] HΦ".
   iNamed "Hclerk".
@@ -339,9 +394,8 @@ Proof using Type*.
     iIntros.
     iModIntro; iFrame.
   }
-  wpc_call.
-  { admit. }
-
+  wpc_rec _.
+  { iFromCache. }
 
   iCache with "Hprecond HΦ".
   { (* Use PreCond to show idemp_fupd *)
@@ -400,12 +454,15 @@ Proof using Type*.
   { by iNamedAccu. }
   {
     iNamed 1.
-    admit.
+    iDestruct "HΦ" as "[HΦc _]".
+    iModIntro.
+    iApply "HΦc".
+    admit. (* TODO: Use quiesce_request *)
   }
   {
     iIntros "!# __CTX"; iNamed "__CTX".
-    admit.
-  }
+
+    wpc_pures.
   (*
   iDestruct "Herrb_ptr" as (err_old) "Herrb_ptr".
   wp_pures.
